more

backends/lean/Aeneas/Std/Scalar/OverflowingOps.lean
@@ -1,5 +1,6 @@
 import Aeneas.Std.Scalar.Core
 import Aeneas.Std.Scalar.Elab
+import Aeneas.Tactic.Solver.ScalarTac.Lemmas
 
 namespace Aeneas.Std
 
@@ -11,55 +12,44 @@ open ScalarElab
 
 -- TODO: we should redefine this, in particular so that it doesn't live in the `Result` monad
 
-def UScalar.overflowing_add {ty} (x y : UScalar ty) : UScalar ty × Bool :=
-  (⟨ BitVec.ofNat _ (x.toNat + y.toNat) ⟩, 2^ty.numBits ≤ x.toNat + y.toNat)
-
-def IScalar.overflowing_add (ty : IScalarTy) (x y : IScalar ty) : IScalar ty × Bool :=
-  (⟨ BitVec.ofInt _ (x.toInt + y.toInt) ⟩,
-     ¬ (-2^(ty.numBits -1) ≤ x.toInt + y.toInt ∧ x.toInt + y.toInt < 2^(ty.numBits-1)))
-
 /- [core::num::{u8}::overflowing_add] -/
-uscalar def core.num.«%S».overflowing_add := @UScalar.overflowing_add .«%S»
+uscalar def core.num.«%S».overflowing_add (x y : «%S») : «%S» × Bool :=
+  (⟨ BitVec.ofNat _ (x.toNat + y.toNat) ⟩, 2^«%S».numBits ≤ x.toNat + y.toNat)
 
 /- [core::num::{i8}::overflowing_add] -/
-iscalar def core.num.«%S».overflowing_add := @IScalar.overflowing_add .«%S»
+iscalar def core.num.«%S».overflowing_add (x y : «%S») : «%S» × Bool :=
+  (⟨ BitVec.ofInt _ (x.toInt + y.toInt) ⟩,
+     ¬ (-2^(«%S».numBits -1) ≤ x.toInt + y.toInt ∧ x.toInt + y.toInt < 2^(«%S».numBits-1)))
 
 attribute [-simp] Bool.exists_bool
 
-theorem UScalar.overflowing_add_eq {ty} (x y : UScalar ty) :
-  let z := overflowing_add x y
-  if x.toNat + y.toNat > UScalar.max ty then
-    z.fst.toNat + UScalar.size ty = x.toNat + y.toNat ∧
+uscalar @[step_pure overflowing_add x y]
+theorem core.num.«%S».overflowing_add_eq (x y : «%S») :
+  let z := core.num.«%S».overflowing_add x y
+  if x.toNat + y.toNat > «%S».max then
+    z.fst.toNat + «%S».size = x.toNat + y.toNat ∧
     z.snd = true
   else
     z.fst.toNat = x.toNat + y.toNat ∧
     z.snd = false
   := by
-  simp [overflowing_add]
-  simp only [toNat, BitVec.toNat_ofNat, max]
+  simp [core.num.«%S».overflowing_add]
+  simp only [UScalar.toNat, «%S».numBits_eq, UScalarTy.numBits, BitVec.toNat_ofNat, max]
   split <;> rename_i hLt
   . split_conjs
-    . have : (x.toBitVec.toNat + y.toBitVec.toNat) % 2^ty.numBits =
-             (x.toBitVec.toNat + y.toBitVec.toNat - 2^ty.numBits) % 2^ty.numBits := by
+    . have : (x.toBitVec.toNat + y.toBitVec.toNat) % 2^%BitWidth =
+             (x.toBitVec.toNat + y.toBitVec.toNat - 2^%BitWidth) % 2^%BitWidth := by
         rw [Nat.mod_eq_sub_mod]
-        omega
+        scalar_tac
       rw [this]; clear this
-
-      have := @Nat.mod_eq_of_lt (x.toBitVec.toNat + y.toBitVec.toNat - 2^ty.numBits) (2^ty.numBits) (by omega)
+      have := @Nat.mod_eq_of_lt (x.toBitVec.toNat + y.toBitVec.toNat - 2^%BitWidth) (2^%BitWidth) (by omega)
       rw [this]; clear this
-      simp [size]
+      simp [«%S».size]
       scalar_tac
-    . omega
+    . scalar_tac
   . split_conjs
     . apply Nat.mod_eq_of_lt
-      omega
-    . omega
-
-uscalar @[step_pure overflowing_add x y]
-theorem core.num.«%S».overflowing_add_eq (x y : «%S») :
-  let z := overflowing_add x y
-  if x.toNat + y.toNat > UScalar.max .«%S» then z.fst.toNat + UScalar.size .«%S» = x.toNat + y.toNat ∧ z.snd = true
-  else z.fst.toNat = x.toNat + y.toNat ∧ z.snd = false
-  := UScalar.overflowing_add_eq x y
+      scalar_tac
+    . scalar_tac
 
 end Aeneas.Std
