backends/lean/Aeneas/Std/RawPtr.lean
@@ -16,17 +16,23 @@ inductive ScalarKind where
 | Signed (ty : IScalarTy)
 | Unsigned (ty : UScalarTy)
 
-class IsScalar (T : Type) where
-  isScalar : (∃ ty, T = UScalar ty) ∨ (∃ ty, T = IScalar ty)
-
-instance {ty} : IsScalar (UScalar ty) where
-  isScalar := by simp
-
-instance {ty} : IsScalar (IScalar ty) where
-  isScalar := by simp
+inductive IsScalar : Type → Prop where
+  | u8    : IsScalar U8
+  | u16   : IsScalar U16
+  | u32   : IsScalar U32
+  | u64   : IsScalar U64
+  | u128  : IsScalar U128
+  | usize : IsScalar Usize
+  | i8    : IsScalar I8
+  | i16   : IsScalar I16
+  | i32   : IsScalar I32
+  | i64   : IsScalar I64
+  | i128  : IsScalar I128
+  | isize : IsScalar Isize
 
 -- TODO: we can properly define this once we have separation logic
-def RawPtr.cast_scalar {T} {M} (T' : Type) (M' : Mutability) [IsScalar T] [IsScalar T'] (_ : RawPtr T M) :
+def RawPtr.cast_scalar {T} {M} (T' : Type) (M' : Mutability)
+    (_hT : IsScalar T) (_hT' : IsScalar T') (_ : RawPtr T M) :
   Result (RawPtr T' M') :=
   .fail .undef
 
